insertNotFound seems ok

concurrency/disciplined/sharedexclusive-linearatomic/CircularTable.i.dfy
@@ -194,7 +194,13 @@ module CircularTable {
       :: SlotShouldSkip(table[i], i, key))
   }
 
-  predicate ValidProbeRange(table: FixedTable, key: Key, range: Range)
+  predicate KeyPresentProbeRange(table: FixedTable, key: Key, range: Range)
+  {
+    && ValidPartialProbeRange(table, key, range)
+    && SlotFullWithKey(table[range.end], key)
+  }
+
+  predicate KeyAbsentProbeRange(table: FixedTable, key: Key, range: Range)
   {
     // skip upto (not including) end
     && ValidPartialProbeRange(table, key, range)
@@ -207,7 +213,7 @@ module CircularTable {
   // a valid probe range would cover key's hash segment 
   lemma ProbeRangeSufficient(table: FixedTable, key: Key, p_range: Range)
     requires TableInv(table)
-    requires ValidProbeRange(table, key, p_range)
+    requires KeyAbsentProbeRange(table, key, p_range)
     ensures var h_range := GetHashSegment(table, hash(key));
       h_range.HasSome() ==> (
         && p_range.Contains(h_range.start)
@@ -276,231 +282,6 @@ module CircularTable {
   predicate RangeKnown(table: FixedTable, range: Range)
   {
     forall i: Index | range.Contains(i) :: table[i].Some?
-  }
-
-  function {:fuel 1} UnwrapRange(table: FixedTable, range: Range): (s: seq<Entry>)
-    requires RangeKnown(table, range)
-    ensures |range| == |s|
-    decreases |range|
-  {
-    if range.HasNone() then
-      assert |range| == 0;
-      []
-    else
-      var last := range.GetLast();
-      UnwrapRange(table, range.RightShrink1()) + [table[last].value]
-  }
-
-  lemma UnwrapRangeIndex(table: FixedTable, r1: Range, entries: seq<Entry>)
-    requires r1.Partial?
-    requires RangeKnown(table, r1) 
-    requires UnwrapRange(table, r1) == entries
-    ensures forall i: Index :: r1.Contains(i) ==>  
-      table[i].value == entries[LeftShift(i, r1.start)]
-    ensures forall j: Index :: 0 <= j < |entries| ==> 
-      entries[j] == table[RightShift(r1.start, j)].value
-    decreases |r1|
-  {
-    if r1.HasSome() {
-      UnwrapRangeIndex(table, r1.RightShrink1(), DropLast(entries));
-    }
-  }
-
-  // lemma UnwrapRangeSingleton(table: FixedTable, r1: Range, i: Index)
-  //   requires r1.Partial?
-  //   requires RangeKnown(table, r1) 
-  //   requires r1.Contains(i)
-  // {
-  //   var entries := UnwrapRange(table, r1);
-  //   UnwrapRangeIndex(table, r1, entries);
-  //   assert UnwrapRange(table, Partial(i, NextIndex(i))) == [table[i].value];
-  // }
-
-  lemma UnwrapSplitRange(table: FixedTable, r1: Range, i: Index)
-    requires r1.Partial?
-    requires r1.Contains(i) || i == r1.end
-    requires RangeKnown(table, r1)
-    ensures UnwrapRange(table, r1) == 
-        UnwrapRange(table, Partial(r1.start, i)) +
-        UnwrapRange(table, Partial(i, r1.end))
-    decreases if i == r1.end then 0 else 
-      WrappedDistance(i, r1.end), |r1|
-  {
-    if |r1| == 1 {
-      return;
-    }
-
-    if i == r1.end || i == r1.start {
-      return;
-    }
-
-    var t := UnwrapRange(table, r1);
-    var j := NextIndex(i);
-    var tj1 := UnwrapRange(table, Partial(r1.start, j));
-    var tj2 := UnwrapRange(table, Partial(j, r1.end));
-    var ti1 := UnwrapRange(table, Partial(r1.start, i));
-    var ti2 := UnwrapRange(table, Partial(i, r1.end));
-
-    assert t == tj1 + tj2 by {
-      UnwrapSplitRange(table, r1, j);
-    }
-
-    assert ti1 + [table[i].value] == tj1;
-
-    assert ti2 == UnwrapRange(table, Partial(i, j)) + tj2 by {
-      UnwrapSplitRange(table, Partial(i, r1.end), j);
-    }
-
-    assert UnwrapRange(table, Partial(i, j)) == [table[i].value];
-    // UnwrapRangeSingleton(table, r1, i);
-  }
-
-  lemma UnwrapPrefixRange(table: FixedTable, r1: Range, r2: Range, entries: seq<Entry>)
-    requires r1.Partial? && r2.Partial?
-    requires r1.start == r2.start
-    requires r1.Contains(r2.end)
-    requires RangeKnown(table, r1) 
-    requires UnwrapRange(table, r1) == entries
-    ensures UnwrapRange(table, r2) == entries[ ..|r2| ]
-    decreases |r2|
-  {
-    if |r2| == 0 {
-      return;
-    }
-
-    var entries2 := UnwrapRange(table, r2);
-    var last := r2.GetLast();
-    var r3 := r2.RightShrink1();
-    var l2, l3 := |r2|, |r3|;
-
-    calc {
-      UnwrapRange(table, r2);
-      UnwrapRange(table, r3) + [table[last].value];
-      {
-        UnwrapPrefixRange(table, r1, r3, entries);
-      }
-      entries[..l3] + [table[last].value];
-      {
-        assert entries[l3] == table[last].value by {
-          UnwrapRangeIndex(table, r1, entries);
-          assert last == RightShift(r1.start, l3); 
-        }
-      }
-      entries[..l3] + [entries[l3]];
-      {
-        assert entries[ ..l3] + [entries[l3]] == entries[..l2];
-      }
-      entries[..l2];
-    }
-  }
-
-  lemma UnwrapSuffixRange(table: FixedTable, r1: Range, r2: Range, entries: seq<Entry>)
-    requires r1.Partial? && r2.Partial?
-    requires r1.end == r2.end
-    requires r1.Contains(r2.start) || r2.start == r1.end
-    requires RangeKnown(table, r1) 
-    requires UnwrapRange(table, r1) == entries
-    ensures UnwrapRange(table, r2) == entries[ |entries| - |r2| .. ]
-  {
-    if r2.start == r1.end {
-      return;
-    }
-
-    var entries2 := UnwrapRange(table, r2);
-    var split := r2.start;
-    var r3 := Partial(r1.start, split);
-
-    assert UnwrapRange(table, r1) == 
-      UnwrapRange(table, r3) +
-      UnwrapRange(table, r2) by {
-      UnwrapSplitRange(table, r1, split);
-    }
-
-    assert UnwrapRange(table, r3) == entries[ ..|r3| ] by {
-      UnwrapPrefixRange(table, r1, r3, entries);
-    }
-
-    assert UnwrapRange(table, r2) == entries[ |entries| - |r2| .. ];
-  }
-
-  lemma UnwrapSubRange(table: FixedTable, r1: Range, r2: Range, entries: seq<Entry>)
-    requires r1.Partial? && r2.Partial?
-    requires r1.Contains(r2.start)
-    requires r1.Contains(r2.end) || r2.end == r1.end
-    requires Partial(r1.start, r2.end).Contains(r2.start) || r2.start == r2.end
-
-    requires RangeKnown(table, r1) 
-    requires UnwrapRange(table, r1) == entries
-    ensures UnwrapRange(table, r2) ==
-      entries[WrappedDistance(r1.start, r2.start) ..
-        |entries| - WrappedDistance(r2.end, r1.end)];
-  {
-    var Partial(s1, e1) := r1;
-    var Partial(s2, e2) := r2;
-
-    var t2 := UnwrapRange(table, Partial(s1, s2));
-    var t3 := UnwrapRange(table, r2);
-    var t4 := UnwrapRange(table, Partial(e2, e1));
-
-    assert entries == t2 + t3 + t4 by {
-      UnwrapSplitRange(table, Partial(s1, e2), s2);
-      UnwrapSplitRange(table, r1, e2);
-    }
-
-    assert t2 == entries[..|t2| ] by {
-      UnwrapPrefixRange(table, r1, Partial(s1, s2), entries);
-    }
-
-    assert t4 == entries[ |entries| - |t4| .. ] by {
-      UnwrapSuffixRange(table, r1, Partial(e2, e1), entries);
-    }
-
-    assert t3 == entries[ |t2| .. |entries| - |t4| ];
-
-    assert |t2| == WrappedDistance(r1.start, r2.start);
-    assert |t4| == WrappedDistance(r2.end, r1.end);
-  }
-
-  lemma RangeEquivalentUnwrap(t1: FixedTable, t2: FixedTable, range: Range)
-    requires RangeEquivalent(t1, t2, range)
-    requires forall i: Index :: range.Contains(i) ==> t1[i].Some?
-    ensures UnwrapRange(t1, range) == UnwrapRange(t2, range)
-    decreases |range|
-  {
-    if range.HasSome() {
-      var last := range.GetLast();
-      assert t1[last] == t2[last];
-      var range' := range.RightShrink1();
-      RangeEquivalentUnwrap(t1, t2, range');
-    } 
-  }
-
-  predicate RangeRightShift1Equivalent(t1: FixedTable, t2: FixedTable, r: Range)
-  {
-    forall i: Index :: r.Contains(i) ==> t1[i] == t2[NextIndex(i)]
-  }
-
-  lemma RangeShiftEquivalentUnwrap(t1: FixedTable, t2: FixedTable, r1: Range)
-    requires r1.Partial?
-    requires RangeRightShift1Equivalent(t1, t2, r1)
-    requires forall i: Index :: r1.Contains(i) ==> t1[i].Some?
-    ensures forall i: Index :: r1.RightShift1().Contains(i) ==> t2[i].Some?
-    ensures UnwrapRange(t1, r1) == UnwrapRange(t2, r1.RightShift1())
-    decreases |r1|
-  {
-    var r2 := r1.RightShift1();
-    if r1.HasSome() {
-      forall i: Index | r2.Contains(i)
-        ensures t2[i] == t1[PrevIndex(i)]
-      {
-        assert r1.Contains(PrevIndex(i));
-      }
-
-      var last := r1.GetLast();
-      assert t1[last] == t2[NextIndex(last)];
-      var r1' := r1.RightShrink1();
-      RangeShiftEquivalentUnwrap(t1, t2, r1');
-    }
   }
 
 //////////////////////////////////////////////////////////////////////////////
@@ -771,54 +552,6 @@ module CircularTable {
       TableQuantityConcat5([table[last_index]], table[..end], table[end+1..start], [inserted], table[start..last_index]);
       TableQuantityConcat5(table[..end], [table[end]], table[end+1..start], table[start..last_index], [table[last_index]]);
     }
-  }
-
-  lemma RightShiftUnwrap(t1: FixedTable, t2: FixedTable,
-    inserted: Entry, entries: seq<Entry>,
-    range: Range, start: Index)
-    requires range.Partial?
-    requires range.Contains(start)
-    requires RangeKnown(t1, range)
-    requires UnwrapRange(t1, range) == entries
-    requires IsTableRightShift(t1, t2, Some(inserted), start, PrevIndex(range.end))
-    ensures var probe_len := WrappedDistance(range.start, start);
-      UnwrapRange(t2, range) == entries[..probe_len] + [inserted] + entries[probe_len..|entries| - 1];
-  {
-    var end := PrevIndex(range.end);
-    var probe_range := Partial(range.start, start);
-    var probe_len := |probe_range|;
-    var shift_range := Partial(start, end);
-    var len := |range|;
-
-    assert UnwrapRange(t1, range) == entries;
-
-    assert UnwrapRange(t2, probe_range) == entries[..probe_len] by {
-      assert RangeEquivalent(t1, t2, probe_range);
-      RangeEquivalentUnwrap(t1, t2, probe_range);
-      UnwrapPrefixRange(t1, range, probe_range, entries);
-      // assert UnwrapRange(t1, probe_range) == UnwrapRange(t2, probe_range);
-    }
-
-    assert UnwrapRange(t2, shift_range.RightShift1()) == entries[probe_len..len - 1] by {
-      RangeShiftEquivalentUnwrap(t1, t2, shift_range);
-      UnwrapSubRange(t1, range, shift_range, entries);
-      // assert UnwrapRange(t1, shift_range) == UnwrapRange(t2, shift_range.RightShift1());
-    }
-
-    var start_next := NextIndex(start);
-    
-    assert UnwrapRange(t2, range) == UnwrapRange(t2, probe_range)
-      + UnwrapRange(t2, Partial(start, start_next))
-      + UnwrapRange(t2, shift_range.RightShift1()) by {
-      UnwrapSplitRange(t2, range, start_next);
-      UnwrapSplitRange(t2, Partial(range.start, start_next), start);
-    }
-
-    assert UnwrapRange(t2, Partial(start, start_next)) == [inserted] by {
-      assert t2[start] == Some(inserted);
-    }
-
-    assert UnwrapRange(t2, range) == entries[..probe_len] + [inserted] + entries[probe_len..len - 1];
   }
 
   predicate IsTableLeftShift(table: FixedTable, table': FixedTable, start: Index, end: Index)
@@ -1137,6 +870,303 @@ module CircularTable {
     
     assert m' == m[inserted.key := inserted.value];
   }
+
+//////////////////////////////////////////////////////////////////////////////
+// unwrapping
+//////////////////////////////////////////////////////////////////////////////
+
+  function {:fuel 1} UnwrapRange(table: FixedTable, range: Range): (s: seq<Entry>)
+    requires RangeKnown(table, range)
+    ensures |range| == |s|
+    decreases |range|
+  {
+    if range.HasNone() then
+      assert |range| == 0;
+      []
+    else
+      var last := range.GetLast();
+      UnwrapRange(table, range.RightShrink1()) + [table[last].value]
+  }
+
+  lemma UnwrapRangeIndex(table: FixedTable, r1: Range, entries: seq<Entry>)
+    requires r1.Partial?
+    requires RangeKnown(table, r1) 
+    requires UnwrapRange(table, r1) == entries
+    ensures forall i: Index :: r1.Contains(i) ==>  
+      table[i].value == entries[LeftShift(i, r1.start)]
+    ensures forall j: Index :: 0 <= j < |entries| ==> 
+      entries[j] == table[RightShift(r1.start, j)].value
+    decreases |r1|
+  {
+    if r1.HasSome() {
+      UnwrapRangeIndex(table, r1.RightShrink1(), DropLast(entries));
+    }
+  }
+
+  // lemma UnwrapRangeSingleton(table: FixedTable, r1: Range, i: Index)
+  //   requires r1.Partial?
+  //   requires RangeKnown(table, r1) 
+  //   requires r1.Contains(i)
+  // {
+  //   var entries := UnwrapRange(table, r1);
+  //   UnwrapRangeIndex(table, r1, entries);
+  //   assert UnwrapRange(table, Partial(i, NextIndex(i))) == [table[i].value];
+  // }
+
+  lemma UnwrapSplitRange(table: FixedTable, r1: Range, i: Index)
+    requires r1.Partial?
+    requires r1.Contains(i) || i == r1.end
+    requires RangeKnown(table, r1)
+    ensures UnwrapRange(table, r1) == 
+        UnwrapRange(table, Partial(r1.start, i)) +
+        UnwrapRange(table, Partial(i, r1.end))
+    decreases if i == r1.end then 0 else 
+      WrappedDistance(i, r1.end), |r1|
+  {
+    if |r1| == 1 {
+      return;
+    }
+
+    if i == r1.end || i == r1.start {
+      return;
+    }
+
+    var t := UnwrapRange(table, r1);
+    var j := NextIndex(i);
+    var tj1 := UnwrapRange(table, Partial(r1.start, j));
+    var tj2 := UnwrapRange(table, Partial(j, r1.end));
+    var ti1 := UnwrapRange(table, Partial(r1.start, i));
+    var ti2 := UnwrapRange(table, Partial(i, r1.end));
+
+    assert t == tj1 + tj2 by {
+      UnwrapSplitRange(table, r1, j);
+    }
+
+    assert ti1 + [table[i].value] == tj1;
+
+    assert ti2 == UnwrapRange(table, Partial(i, j)) + tj2 by {
+      UnwrapSplitRange(table, Partial(i, r1.end), j);
+    }
+
+    assert UnwrapRange(table, Partial(i, j)) == [table[i].value];
+    // UnwrapRangeSingleton(table, r1, i);
+  }
+
+  lemma UnwrapPrefixRange(table: FixedTable, r1: Range, r2: Range, entries: seq<Entry>)
+    requires r1.Partial? && r2.Partial?
+    requires r1.start == r2.start
+    requires r1.Contains(r2.end)
+    requires RangeKnown(table, r1) 
+    requires UnwrapRange(table, r1) == entries
+    ensures UnwrapRange(table, r2) == entries[ ..|r2| ]
+    decreases |r2|
+  {
+    if |r2| == 0 {
+      return;
+    }
+
+    var entries2 := UnwrapRange(table, r2);
+    var last := r2.GetLast();
+    var r3 := r2.RightShrink1();
+    var l2, l3 := |r2|, |r3|;
+
+    calc {
+      UnwrapRange(table, r2);
+      UnwrapRange(table, r3) + [table[last].value];
+      {
+        UnwrapPrefixRange(table, r1, r3, entries);
+      }
+      entries[..l3] + [table[last].value];
+      {
+        assert entries[l3] == table[last].value by {
+          UnwrapRangeIndex(table, r1, entries);
+          assert last == RightShift(r1.start, l3); 
+        }
+      }
+      entries[..l3] + [entries[l3]];
+      {
+        assert entries[ ..l3] + [entries[l3]] == entries[..l2];
+      }
+      entries[..l2];
+    }
+  }
+
+  lemma UnwrapSuffixRange(table: FixedTable, r1: Range, r2: Range, entries: seq<Entry>)
+    requires r1.Partial? && r2.Partial?
+    requires r1.end == r2.end
+    requires r1.Contains(r2.start) || r2.start == r1.end
+    requires RangeKnown(table, r1) 
+    requires UnwrapRange(table, r1) == entries
+    ensures UnwrapRange(table, r2) == entries[ |entries| - |r2| .. ]
+  {
+    if r2.start == r1.end {
+      return;
+    }
+
+    var entries2 := UnwrapRange(table, r2);
+    var split := r2.start;
+    var r3 := Partial(r1.start, split);
+
+    assert UnwrapRange(table, r1) == 
+      UnwrapRange(table, r3) +
+      UnwrapRange(table, r2) by {
+      UnwrapSplitRange(table, r1, split);
+    }
+
+    assert UnwrapRange(table, r3) == entries[ ..|r3| ] by {
+      UnwrapPrefixRange(table, r1, r3, entries);
+    }
+
+    assert UnwrapRange(table, r2) == entries[ |entries| - |r2| .. ];
+  }
+
+  lemma UnwrapSubRange(table: FixedTable, r1: Range, r2: Range, entries: seq<Entry>)
+    requires r1.Partial? && r2.Partial?
+    requires r1.Contains(r2.start)
+    requires r1.Contains(r2.end) || r2.end == r1.end
+    requires Partial(r1.start, r2.end).Contains(r2.start) || r2.start == r2.end
+
+    requires RangeKnown(table, r1) 
+    requires UnwrapRange(table, r1) == entries
+    ensures UnwrapRange(table, r2) ==
+      entries[WrappedDistance(r1.start, r2.start) ..
+        |entries| - WrappedDistance(r2.end, r1.end)];
+  {
+    var Partial(s1, e1) := r1;
+    var Partial(s2, e2) := r2;
+
+    var t2 := UnwrapRange(table, Partial(s1, s2));
+    var t3 := UnwrapRange(table, r2);
+    var t4 := UnwrapRange(table, Partial(e2, e1));
+
+    assert entries == t2 + t3 + t4 by {
+      UnwrapSplitRange(table, Partial(s1, e2), s2);
+      UnwrapSplitRange(table, r1, e2);
+    }
+
+    assert t2 == entries[..|t2| ] by {
+      UnwrapPrefixRange(table, r1, Partial(s1, s2), entries);
+    }
+
+    assert t4 == entries[ |entries| - |t4| .. ] by {
+      UnwrapSuffixRange(table, r1, Partial(e2, e1), entries);
+    }
+
+    assert t3 == entries[ |t2| .. |entries| - |t4| ];
+
+    assert |t2| == WrappedDistance(r1.start, r2.start);
+    assert |t4| == WrappedDistance(r2.end, r1.end);
+  }
+
+  lemma RangeEquivalentUnwrap(t1: FixedTable, t2: FixedTable, range: Range)
+    requires RangeEquivalent(t1, t2, range)
+    requires forall i: Index :: range.Contains(i) ==> t1[i].Some?
+    ensures UnwrapRange(t1, range) == UnwrapRange(t2, range)
+    decreases |range|
+  {
+    if range.HasSome() {
+      var last := range.GetLast();
+      assert t1[last] == t2[last];
+      var range' := range.RightShrink1();
+      RangeEquivalentUnwrap(t1, t2, range');
+    } 
+  }
+
+  predicate RangeRightShift1Equivalent(t1: FixedTable, t2: FixedTable, r: Range)
+  {
+    forall i: Index :: r.Contains(i) ==> t1[i] == t2[NextIndex(i)]
+  }
+
+  lemma RangeShiftEquivalentUnwrap(t1: FixedTable, t2: FixedTable, r1: Range)
+    requires r1.Partial?
+    requires RangeRightShift1Equivalent(t1, t2, r1)
+    requires forall i: Index :: r1.Contains(i) ==> t1[i].Some?
+    ensures forall i: Index :: r1.RightShift1().Contains(i) ==> t2[i].Some?
+    ensures UnwrapRange(t1, r1) == UnwrapRange(t2, r1.RightShift1())
+    decreases |r1|
+  {
+    var r2 := r1.RightShift1();
+    if r1.HasSome() {
+      forall i: Index | r2.Contains(i)
+        ensures t2[i] == t1[PrevIndex(i)]
+      {
+        assert r1.Contains(PrevIndex(i));
+      }
+
+      var last := r1.GetLast();
+      assert t1[last] == t2[NextIndex(last)];
+      var r1' := r1.RightShrink1();
+      RangeShiftEquivalentUnwrap(t1, t2, r1');
+    }
+  }
+
+  lemma RightShiftUnwrap(t1: FixedTable, t2: FixedTable,
+    inserted: Entry, entries: seq<Entry>,
+    range: Range, start: Index)
+    requires range.Partial?
+    requires range.Contains(start)
+    requires RangeKnown(t1, range)
+    requires UnwrapRange(t1, range) == entries
+    requires IsTableRightShift(t1, t2, Some(inserted), start, PrevIndex(range.end))
+    ensures var probe_len := WrappedDistance(range.start, start);
+      UnwrapRange(t2, range) == entries[..probe_len] + [inserted] + entries[probe_len..|entries| - 1];
+  {
+    var end := PrevIndex(range.end);
+    var probe_range := Partial(range.start, start);
+    var shift_range := Partial(start, end);
+    var probe_len := |probe_range|;
+    var len := |range|;
+
+    assert UnwrapRange(t1, range) == entries;
+
+    assert UnwrapRange(t2, probe_range) == entries[..probe_len] by {
+      assert RangeEquivalent(t1, t2, probe_range);
+      RangeEquivalentUnwrap(t1, t2, probe_range);
+      UnwrapPrefixRange(t1, range, probe_range, entries);
+      // assert UnwrapRange(t1, probe_range) == UnwrapRange(t2, probe_range);
+    }
+
+    assert UnwrapRange(t2, shift_range.RightShift1()) == entries[probe_len..len - 1] by {
+      RangeShiftEquivalentUnwrap(t1, t2, shift_range);
+      UnwrapSubRange(t1, range, shift_range, entries);
+      // assert UnwrapRange(t1, shift_range) == UnwrapRange(t2, shift_range.RightShift1());
+    }
+
+    var start_next := NextIndex(start);
+    
+    assert UnwrapRange(t2, range) == UnwrapRange(t2, probe_range)
+      + UnwrapRange(t2, Partial(start, start_next))
+      + UnwrapRange(t2, shift_range.RightShift1()) by {
+      UnwrapSplitRange(t2, range, start_next);
+      UnwrapSplitRange(t2, Partial(range.start, start_next), start);
+    }
+
+    assert UnwrapRange(t2, Partial(start, start_next)) == [inserted] by {
+      assert t2[start] == Some(inserted);
+    }
+
+    assert UnwrapRange(t2, range) == entries[..probe_len] + [inserted] + entries[probe_len..len - 1];
+  }
+
+  // lemma OverwriteUnwrap(t1: FixedTable, t2: FixedTable,
+  //   inserted: Entry, entries: seq<Entry>,
+  //   range: Range, start: Index)
+  //   requires range.Partial?
+  //   requires range.Contains(start)
+  //   requires RangeKnown(t1, range)
+  //   requires UnwrapRange(t1, range) == entries
+  //   requires t2 == t1[start := Some(inserted)]
+  // {
+  //   var probe_range := Partial(range.start, start);
+  //   var probe_len := |probe_range|;
+
+  //   assert UnwrapRange(t2, probe_range) == entries[..probe_len] by {
+  //     assert RangeEquivalent(t1, t2, probe_range);
+  //     RangeEquivalentUnwrap(t1, t2, probe_range);
+  //     UnwrapPrefixRange(t1, range, probe_range, entries);
+  //   }
+  // }
+
 }
   // lemma ValidHashSegmentsImpliesDisjoint(table: FixedTable, h0: Index, h1: Index)
   //   requires h0 != h1
